Defined proofs. Buggy checker. Started proof.

logic.v
@@ -38,7 +38,7 @@ Fixpoint member (f:formula) (C:context) : Prop :=
     | p::rest => if formula_dec f p then True else member f rest
   end.
 
-Fixpoint subst (a:pcpl) (f:formula) (n:nat) : formula :=
+Fixpoint subst (a:pcpl) (f:formula) (n:var) : formula :=
   match f with
     | Pred_f s (Var_p v) => if eq_nat_dec v n 
                               then Pred_f s (Pcpl_p a)
@@ -105,15 +105,125 @@ Ltac prove_auth :=
     | [ |- _ |-- _] => try (econstructor ; simpl ; auto)
   end.
 
-Ltac spec_auth p := eapply (Spec_e _ p _ _ _) ; simpl ; repeat prove_auth.
+Ltac spec_auth p := eapply (Spec_e _ p _ _ _) ; simpl.
 
 Lemma test : (delegate "a" "b" "ok")::(Signed_f (Pcpl_p "b") (Pred_f "ok" (Pcpl_p "c")))::nil |-- Says_f (Pcpl_p "a") (Pred_f "ok" (Pcpl_p "c")).
 Proof.
-  unfold delegate ; repeat prove_auth; spec_auth "c".
+  Show.
+  unfold delegate ; repeat prove_auth; spec_auth "c" ; repeat prove_auth.
+Qed.
+
+Lemma says : Signed_f (Pcpl_p "a") (Pred_f "p" (Pcpl_p "a"))::nil  |-- Says_f (Pcpl_p "a") (Pred_f "p" (Pcpl_p "a")).
+Proof.
+ Show.
+ apply Signed_e.
+ apply Tauto_e.
+ apply Init_e.
+ simpl. auto.
 Qed.
 
 (** Define a data structure for proofs *)
+Inductive proof : Set :=
+ | Signed_r : formula -> proof (* formula = Signed_f f *)
+ | Confirms_r : formula -> proof (* formula = Confirms_f f *)
+ | Tauto_r : formula -> proof -> proof (* formula = Says_f a f, proof of f *) 
+(* | Weaken_r : formula -> proof -> proof *)
+ | Impl_r : formula -> proof -> proof -> proof -> proof (* formula = f3, proof of f1, f1->f2, f2->f3 *)
+ | Says_Confirms_r : formula -> proof -> proof -> proof (* formula = Says_f a f2, proof of Confirms_f a f1, f1->Says_f a f2 *) 
+ | Says_Signed_r : formula -> proof -> proof -> proof (* formula = Says_f a f2, proof of Signed_f a f1, f1->Says_f a f2 *) 
+ | Says_Says_r : formula -> proof -> proof -> proof (* formula = Says_f a f2, proof of Says_f a f1, f1->Says_f a f2 *) 
+ | Says_Spec_r : formula -> pcpl -> proof -> proof -> proof. (* formula = Says_f a f2, principal = p, proof of Abs_f f1, subst p f1 0 -> Says_f a f2 *)
 
 (** Define a proof checking function (Fixpoint check : formula -> proof -> Prop) *)
 
-(** Prove that check f p -> nil |- f *)
+Definition proof_goal p : formula :=
+match p with
+  | Signed_r f => f
+  | Confirms_r f => f
+  | Tauto_r f _ => f
+  | Impl_r f _ _ _ => f
+  | Says_Confirms_r f _ _ => f 
+  | Says_Signed_r f _ _ => f
+  | Says_Says_r f _ _ => f
+  | Says_Spec_r f _ _ _ => f
+end.
+
+Fixpoint check (g:formula) (p:proof) : Prop :=
+  match p with
+    | Signed_r f => match f with
+                      | Signed_f _ _ => if formula_dec f g then True else False
+                      | _ => False
+                    end
+    | Confirms_r f => match f with
+                      | Confirms_f _ _ => if formula_dec f g then True else False
+                      | _ => False
+                      end
+    | Tauto_r f p1 => match f with
+                        | Says_f _ f2 => if formula_dec f g then check f2 p1 else False
+                        | _ => False
+                      end
+    | Impl_r f p1 p2 p3 => match proof_goal p2 with
+                             | Impl_f f1 f2 => check f1 p1 /\ check (Impl_f f1 f2) p2 /\ check (Impl_f f2 f) p3
+                             | _ => False
+                           end
+    | Says_Confirms_r f p1 p2 => match f with
+                                   | Says_f a f2 => match proof_goal p1 with
+                                                      | Confirms_f a f1 => check (Confirms_f a f1) p1 /\ check (Impl_f f1 f) p2
+                                                      | _ => False
+                                                    end
+                                   | _ => False
+                                 end
+    | Says_Signed_r f p1 p2 => match f with
+                                   | Says_f a f2 => match proof_goal p1 with
+                                                      | Signed_f a f1 => check (Signed_f a f1) p1 /\ check (Impl_f f1 f) p2
+                                                      | _ => False
+                                                    end
+                                   | _ => False
+                                 end
+    | Says_Says_r f p1 p2 =>  match f with
+                                   | Says_f a f2 => match proof_goal p1 with
+                                                      | Says_f a f1 => check (Says_f a f1) p1 /\ check (Impl_f f1 f) p2
+                                                      | _ => False
+                                                    end
+                                   | _ => False
+                                 end
+    | Says_Spec_r f theP p1 p2 => match f with
+                                    | Says_f a f2 => match proof_goal p1 with
+                                                       | Abs_f f1 => check (Abs_f f1) p1 /\ check (Impl_f (subst theP f1 0) f) p2
+                                                       | _ => False
+                                                     end
+                                    | _ => False
+                                  end
+  end.
+
+Fixpoint axioms (p:proof) : context :=
+match p with
+  | Signed_r f => f::nil
+  | Confirms_r f => f::nil
+  | Tauto_r f p1 => axioms p1
+  | Impl_r f p1 p2 p3 => List.app (axioms p1) (List.app (axioms p2) (axioms p3))
+  | Says_Confirms_r f p1 p2 => List.app (axioms p1) (axioms p2) 
+  | Says_Signed_r f p1 p2 => List.app (axioms p1) (axioms p2)
+  | Says_Says_r f p1 p2 => List.app (axioms p1) (axioms p2)
+  | Says_Spec_r f _ p1 p2 => List.app (axioms p1) (axioms p2)
+end.
+
+(** Prove that check f p -> (all signed or confirmed things) |- f *)
+
+Lemma foo : forall f1 f2, (if formula_dec f1 f2 then True else False) = (if formula_dec f2 f1 then True else False). 
+Proof.
+  intros ; destruct formula_dec ; destruct formula_dec ; simpl ; congruence.
+Qed.  
+
+Theorem checker_correct : forall f p, check f p -> axioms p |-- f.
+Proof.
+  intros.
+  induction p ; try (simpl in * ; destruct f0 ; try (exfalso ; auto ; fail) ; prove_auth ; try (rewrite foo ; auto) ; fail).
+  assert (axioms (Tauto_r f0 p) = axioms p).
+  simpl ; auto.
+  rewrite H0.
+  simpl in H.
+  destruct f0 ; try (exfalso ; auto ; fail).
+  destruct formula_dec.
+  rewrite e in H0.
+Admitted.
